refocusing_machine_sig.v
@@ -1,16 +1,18 @@
-Require Export refocusing_lang.
-Require Import Program.
+Require Import reduction_semantics.
+Require Export refocusing_step.
+Require Import refocusing_semantics.
+Require Export abstract_machine.
 
 
 
-Module Type PRE_ABSTRACT_MACHINE (R : RED_LANG).
 
-  Declare Module DEC : DEC_STEP R.
+Module Type PRE_ABSTRACT_MACHINE (R : RED_LANG) (RS : RED_REF_SEM R).
+
+  Module DEC := RS.DEC.
   Import R.
   Export DEC.
 
 
-  (** A decomposition function specified in terms of the atomic functions above *)
   Inductive dec : term -> forall {k1 k2}, context k1 k2 -> decomp k1 -> Prop :=
 
   | d_dec  : forall t {k1 k2} (c : context k1 k2) {r},
@@ -45,27 +47,31 @@ Module Type PRE_ABSTRACT_MACHINE (R : RED_LANG).
                 dec t (ec0=:c) d ->
                 decctx v (ec=:c) d.
 
-  Scheme dec_Ind := Induction for dec Sort Prop
+  Scheme dec_Ind    := Induction for dec Sort Prop
     with decctx_Ind := Induction for decctx Sort Prop.
 
 
   Inductive iter : forall {k}, decomp k -> value k -> Prop :=
-  | i_val : forall {k} (v : value k), iter (d_val v) v
+  | i_val : forall {k} (v : value k), 
+              iter (d_val v) v
   | i_red : forall {k2} (r : redex k2) {t k1} {c : context k1 k2} {d v},
-              contract r = Some t -> dec t c d -> iter d v ->
+              contract r = Some t -> 
+              dec t c d -> 
+              iter d v ->
               iter (d_red r c) v.
 
+
   Inductive eval : term -> value init_ckind -> Prop :=
-  | e_intro : forall {t} {d : decomp init_ckind} {v : value init_ckind},
-                dec t [.] d -> iter d v -> eval t v.
+  | e_intro : forall {t d v}, dec t [.] d -> iter d v -> eval t v.
 
 End PRE_ABSTRACT_MACHINE.
 
 
 
-Module Type STAGED_ABSTRACT_MACHINE (R : RED_LANG).
 
-  Declare Module DEC : DEC_STEP R.
+Module Type STAGED_ABSTRACT_MACHINE (R : RED_LANG) (RS : RED_REF_SEM R).
+
+  Module DEC := RS.DEC.
   Import R.
   Export DEC.
 
@@ -73,13 +79,16 @@ Module Type STAGED_ABSTRACT_MACHINE (R : RED_LANG).
   Inductive dec : term -> forall {k1 k2}, context k1 k2 -> value k1 -> Prop :=
 
   | d_dec  : forall t {k1 k2} {c : context k1 k2} {r v},
-               dec_term t k2 = in_red r -> iter (d_red r c) v ->
+               dec_term t k2 = in_red r -> 
+               iter (d_red r c) v ->
                dec t c v
   | d_v    : forall t {k1 k2} {c : context k1 k2} {v v0},
-               dec_term t k2 = in_val v -> decctx v c v0 ->
+               dec_term t k2 = in_val v -> 
+               decctx v c v0 ->
                dec t c v0
   | d_many : forall t {t0 ec k1 k2} {c : context k1 k2} {v},
-               dec_term t k2 = in_term t0 ec -> dec t0 (ec=:c) v ->
+               dec_term t k2 = in_term t0 ec -> 
+               dec t0 (ec=:c) v ->
                dec t c v
 
   with decctx : forall {k2}, value k2 -> 
@@ -90,20 +99,26 @@ Module Type STAGED_ABSTRACT_MACHINE (R : RED_LANG).
                 iter (d_val v) v0 ->
                 decctx v [.] v0
   | dc_dec  : forall ec {k2} (v : value (k2+>ec)) {k1} {c : context k1 k2} {r v0},
-                dec_context ec k2 v = in_red r -> iter (d_red r c) v0 ->
+                dec_context ec k2 v = in_red r -> 
+                iter (d_red r c) v0 ->
                 decctx v (ec=:c) v0
   | dc_val  : forall ec {k2} (v : value (k2+>ec)) {v0 k1} {c : context k1 k2} {v1},
-                dec_context ec k2 v = in_val v0 -> decctx v0 c v1 ->
+                dec_context ec k2 v = in_val v0 -> 
+                decctx v0 c v1 ->
                 decctx v (ec=:c) v1
   | dc_term : forall ec {k2} (v : value (k2+>ec)) {t ec0 k1} {c : context k1 k2} {v0},
-                dec_context ec k2 v = in_term t ec0 -> dec t (ec0=:c) v0 ->
+                dec_context ec k2 v = in_term t ec0 -> 
+                dec t (ec0=:c) v0 ->
                 decctx v (ec=:c) v0
 
   with iter : forall {k}, decomp k -> value k -> Prop :=
-  | i_val : forall {k} (v : value k), iter (d_val v) v
+
+  | i_val : forall {k} (v : value k), 
+              iter (d_val v) v
   | i_red : forall {k2} (r : redex k2) {k1} {c : context k1 k2} {t v},
-               contract r = Some t -> dec t c v -> 
-               iter (d_red r c) v.
+              contract r = Some t -> 
+              dec t c v -> 
+              iter (d_red r c) v.
 
   Scheme dec_Ind    := Induction for dec Sort Prop
     with decctx_Ind := Induction for decctx Sort Prop
@@ -111,15 +126,16 @@ Module Type STAGED_ABSTRACT_MACHINE (R : RED_LANG).
 
 
   Inductive eval : term -> value init_ckind -> Prop :=
-  | e_intro : forall {t} {v : value init_ckind}, dec t [.] v -> eval t v.
+  | e_intro : forall {t v}, dec t [.] v -> eval t v.
 
 End STAGED_ABSTRACT_MACHINE.
 
 
 
-Module Type EVAL_APPLY_MACHINE (R : RED_LANG).
 
-  Declare Module DEC : DEC_STEP R.
+Module Type EVAL_APPLY_MACHINE (R : RED_LANG) (RS : RED_REF_SEM R).
+
+  Module DEC := RS.DEC.
   Import R.
   Export DEC.
 
@@ -127,13 +143,17 @@ Module Type EVAL_APPLY_MACHINE (R : RED_LANG).
   Inductive dec : term -> forall {k1 k2}, context k1 k2 -> value k1 -> Prop :=
 
   | d_d_r  : forall t {t0 k1 k2} {c : context k1 k2} {r : redex k2} {v},
-               dec_term t k2 = in_red r -> contract r = Some t0 -> dec t0 c v ->
+               dec_term t k2 = in_red r -> 
+               contract r = Some t0 -> 
+               dec t0 c v ->
                dec t c v
   | d_v    : forall t {k1 k2} {c : context k1 k2} {v v0},
-               dec_term t k2 = in_val v -> decctx v c v0 ->
+               dec_term t k2 = in_val v -> 
+               decctx v c v0 ->
                dec t c v0
   | d_term : forall t {t0 ec k1 k2} {c : context k1 k2} {v},
-               dec_term t k2 = in_term t0 ec -> dec t0 (ec=:c) v ->
+               dec_term t k2 = in_term t0 ec -> 
+               dec t0 (ec=:c) v ->
                dec t c v
 
   with decctx : forall {k2}, value k2 -> 
@@ -143,46 +163,52 @@ Module Type EVAL_APPLY_MACHINE (R : RED_LANG).
                ~ dead_ckind k ->
                decctx v [.] v
   | dc_red : forall ec {k2} (v : value (k2+>ec)) {k1} {c : context k1 k2} {r t v0},
-               dec_context ec k2 v = in_red r -> contract r = Some t -> dec t c v0 ->
+               dec_context ec k2 v = in_red r -> 
+               contract r = Some t -> 
+               dec t c v0 ->
                decctx v (ec=:c) v0
   | dc_rec : forall ec {k2} (v : value (k2+>ec)) {k1} {c : context k1 k2} {v0 v1},
-               dec_context ec k2 v = in_val v0 -> decctx v0 c v1 ->
+               dec_context ec k2 v = in_val v0 -> 
+               decctx v0 c v1 ->
                decctx v (ec=:c) v1
   | dc_trm : forall ec {k2} (v : value (k2+>ec)) {k1} {c : context k1 k2} {t ec0 v0},
-               dec_context ec k2 v = in_term t ec0 -> dec t (ec0=:c) v0 ->
+               dec_context ec k2 v = in_term t ec0 -> 
+               dec t (ec0=:c) v0 ->
                decctx v (ec=:c) v0.
 
-
-  Scheme dec_Ind := Induction for dec Sort Prop
+  Scheme dec_Ind    := Induction for dec Sort Prop
     with decctx_Ind := Induction for decctx Sort Prop.
 
 
   Inductive eval : term -> value init_ckind -> Prop :=
-  | e_intro : forall {t} {v : value init_ckind}, dec t [.] v -> eval t v.
+  | e_intro : forall {t v}, dec t [.] v -> eval t v.
 
 End EVAL_APPLY_MACHINE.
 
 
 
-Module Type PROPER_EA_MACHINE (R : RED_LANG).
 
-  Declare Module DEC : DEC_STEP R.
+Module Type PROPER_EA_MACHINE (R : RED_LANG) (RS : RED_REF_SEM R) <: ABSTRACT_MACHINE.
+
   Import R.
-  Export DEC.
+  Import RS.DEC.
 
 
-  Inductive configuration : Set :=
-  | c_eval  : term -> forall {k1 k2}, context k1 k2 -> configuration
-  | c_apply : forall {k1 k2}, context k1 k2 -> value k2 -> configuration.
+  Definition term  := term.
+  Definition value := value init_ckind.
 
-  Definition c_init t                       := c_eval t [.](init_ckind).
-  Definition c_final (v : value init_ckind) := c_apply [.] v.
+  Inductive conf : Set :=
+  | c_eval  : term -> forall {k1 k2}, context k1 k2 -> conf
+  | c_apply : forall {k1 k2}, context k1 k2 -> R.value k2 -> conf.
+  Definition configuration := conf.
+
+  Definition c_init t            := c_eval t [.](init_ckind).
+  Definition c_final (v : value) := c_apply [.] v.
 
 
   Reserved Notation " a → b " (at level 40, no associativity).
 
-
-  Inductive transition : configuration -> configuration -> Prop :=
+  Inductive trans : configuration -> configuration -> Prop :=
 
   | t_red  : forall t {k1 k2} (c : context k1 k2) {r : redex k2} { t0},
                dec_term t k2 = in_red r -> contract r = Some t0 ->
@@ -193,40 +219,46 @@ Module Type PROPER_EA_MACHINE (R : RED_LANG).
   | t_term : forall t {k1 k2} (c : context k1 k2) {t0 ec},
                dec_term t k2 = in_term t0 ec ->
                c_eval t c → c_eval t0 (ec=:c)
-  | t_cred : forall ec {k2} (v : value (k2+>ec)) {k1} (c : context k1 k2) {r t},
+  | t_cred : forall ec {k2} (v : R.value (k2+>ec)) {k1} (c : context k1 k2) {r t},
                dec_context ec k2 v = in_red r -> contract r = Some t ->
                c_apply (ec=:c) v → c_eval t c
-  | t_cval : forall ec {k2} (v : value (k2+>ec)) {k1} (c : context k1 k2) {v0},
+  | t_cval : forall ec {k2} (v : R.value (k2+>ec)) {k1} (c : context k1 k2) {v0},
                dec_context ec k2 v = in_val v0 ->
                c_apply (ec=:c) v → c_apply c v0
-  | t_cterm: forall ec {k2} (v : value (k2+>ec)) {k1} (c : context k1 k2) {t ec0},
+  | t_cterm: forall ec {k2} (v : R.value (k2+>ec)) {k1} (c : context k1 k2) {t ec0},
                dec_context ec k2 v = in_term t ec0 ->
                c_apply (ec=:c) v → c_eval t (ec0=:c)
 
-  where " a → b " := (transition a b).
+  where " a → b " := (trans a b).
+  Definition transition := trans.
+  Hint Unfold transition.
+
+  Inductive trans_close : configuration -> configuration -> Prop :=
+  | one_step   : forall (c0 c1 : configuration), 
+                   transition c0 c1 -> trans_close c0 c1
+  | multi_step : forall (c0 c1 c2 : configuration), 
+                   transition c0 c1 -> trans_close c1 c2 -> trans_close c0 c2.
+  Notation "c0 →+ c1" := (trans_close c0 c1) (at level 40, no associativity).
 
 
-  Declare Module AM : ABSTRACT_MACHINE
-    with Definition term          := term
-    with Definition value         := value init_ckind
-    with Definition configuration := configuration
-    with Definition transition    := transition
-    with Definition c_init        := c_init
-    with Definition c_final       := c_final.
+  Inductive eval : term -> value -> Prop :=
+  | e_intro : forall t v, trans_close (c_init t) (c_final v) -> eval t v.
 
 End PROPER_EA_MACHINE.
 
 
 
-Module Type PUSH_ENTER_MACHINE (R : RED_LANG).
 
-  Declare Module DEC : DEC_STEP R.
+Module Type PUSH_ENTER_MACHINE (R : RED_LANG) (PERS : PE_REF_SEM R).
+
+  Module DEC := PERS.RefSem.DEC.
   Import R.
   Export DEC.
 
 
   Axiom dec_context_not_val : 
-      forall ec {k} v (v0 : value k), dec_context ec k v <> in_val v0.
+      forall ec {k} v1 v0, dec_context ec k v0 <> in_val v1.
+
   Axiom dec_term_value : 
       forall {k} (v : value k), dec_term v k = in_val v.
 
@@ -234,7 +266,9 @@ Module Type PUSH_ENTER_MACHINE (R : RED_LANG).
   Inductive dec : term -> forall {k1 k2}, context k1 k2 -> value k1 -> Prop :=
 
   | dec_r    : forall t {t0 k1 k2} {c : context k1 k2} {r  v},
-                 dec_term t k2 = in_red r -> contract r = Some t0 -> dec t0 c v ->
+                 dec_term t k2 = in_red r -> 
+                 contract r = Some t0 -> 
+                 dec t0 c v ->
                  dec t c v
   | dec_val  : forall t {k} {v : value k},
                  dec_term t k = in_val v ->
@@ -257,42 +291,43 @@ Module Type PUSH_ENTER_MACHINE (R : RED_LANG).
 
 
   Inductive eval : term -> value init_ckind -> Prop :=
-  | e_intro : forall {t} {v : value init_ckind}, dec t [.] v -> eval t v.
+  | e_intro : forall {t v}, dec t [.] v -> eval t v.
 
 End PUSH_ENTER_MACHINE.
 
 
 
-Module Type PROPER_PE_MACHINE (R : RED_LANG).
 
-  Declare Module DEC : DEC_STEP R.
+Module Type PROPER_PE_MACHINE (R : RED_LANG) (PERS : PE_REF_SEM R) <: ABSTRACT_MACHINE.
+
   Import R.
-  Export DEC.
+  Import PERS.RefSem.DEC.
 
 
-  Axiom dec_context_not_val : 
-      forall ec {k} v (v0 : value k), dec_context ec k v <> in_val v0.
-  Axiom dec_term_value : 
-      forall {k} (v : value k), dec_term v k = in_val v.
+  Definition term  := term.
+  Definition value := value init_ckind.
 
 
-  Inductive configuration : Set :=
-  | c_eval  : term -> forall {k1 k2}, context k1 k2 -> configuration
-  | c_final : forall {k}, value k                   -> configuration.
+  Inductive conf : Set :=
+  | c_eval  : term -> forall {k1 k2}, context k1 k2 -> conf
+  | c_fin : forall {k}, R.value k                   -> conf.
+  Definition configuration := conf.
 
-  Definition c_init t := c_eval t [.](init_ckind).
+  Definition c_init t  := c_eval t [.](init_ckind).
+  Definition c_final (v : value) := c_fin v.
 
 
   Reserved Notation " a → b " (at level 40, no associativity).
 
-  Inductive transition : configuration -> configuration -> Prop :=
+  Inductive trans : configuration -> configuration -> Prop :=
 
   | t_red  : forall t {k1 k2} (c : context k1 k2) {t0 r},
-               dec_term t k2 = in_red r -> contract r = Some t0 ->
+               dec_term t k2 = in_red r -> 
+               contract r = Some t0 ->
                c_eval t c → c_eval t0 c
-  | t_cval : forall t {k} {v : value k},
+  | t_cval : forall t {k} {v : R.value k},
                dec_term t k = in_val v ->
-               c_eval t [.](k) → c_final v
+               c_eval t [.](k) → c_fin v
   | t_cred : forall t ec {t0} {k1 k2} (c : context k1 k2) {v r},
                dec_term t (k2+>ec) = in_val v ->
                dec_context ec k2 v = in_red r ->
@@ -306,15 +341,19 @@ Module Type PROPER_PE_MACHINE (R : RED_LANG).
                dec_term t k2 = in_term t0 ec ->
                c_eval t c → c_eval t0 (ec=:c)
 
-  where " a →  b " := (transition a b).
+  where " a →  b " := (trans a b).
+  Definition transition := trans.
+  Hint Unfold transition.
 
 
-  Declare Module AM : ABSTRACT_MACHINE
-    with Definition term          := term
-    with Definition value         := value init_ckind
-    with Definition configuration := configuration
-    with Definition transition    := transition
-    with Definition c_init        := c_init
-    with Definition c_final       := @c_final init_ckind.
+  Inductive trans_close : configuration -> configuration -> Prop :=
+  | one_step   : forall (c0 c1 : configuration), 
+                   transition c0 c1 -> trans_close c0 c1
+  | multi_step : forall (c0 c1 c2 : configuration), 
+                   transition c0 c1 -> trans_close c1 c2 -> trans_close c0 c2.
+  Notation "c0 →+ c1" := (trans_close c0 c1) (at level 40, no associativity).
+
+  Inductive eval : term -> value -> Prop :=
+  | e_intro : forall t v, trans_close (c_init t) (c_final v) -> eval t v.
 
 End PROPER_PE_MACHINE.
