reduction_semantics_facts.v
@@ -1,0 +1,174 @@
+Require Import Util.
+Require Import Program.
+Require Import Eqdep.
+Require Export reduction_semantics.
+
+
+
+
+Module RED_LANG_Facts (R : RED_LANG).
+
+  Import R.
+  
+
+  Lemma ccons_inj : 
+      forall ec {k1 k2} (c : context k1 k2) ec' {k2'} (c' : context k1 k2'), 
+          k2 +> ec = k2' +> ec' -> ec=:c ~= ec'=:c' ->
+          ec = ec' /\ k2 = k2' /\ c ~= c'.
+  Proof.
+    intros.
+    assert (H1 := JMeq_eq_depT _ _ _ _ _ _ H H0).
+    assert (H2 := eq_dep_eq_sigT _ _ _ _ _ _ H1). 
+    inversion H2; subst.
+    dep_subst.
+    auto.
+  Qed.
+
+
+  Lemma death_propagation2 : 
+      forall k ec, ~ dead_ckind (k+>ec) -> ~ dead_ckind k.
+
+  Proof.
+    intuition.
+    apply H.
+    apply death_propagation.
+    assumption.
+  Qed.
+
+
+  Lemma dead_context_dead : 
+      forall {k1 k2}, context k1 k2 -> dead_ckind k1 -> dead_ckind k2.
+
+  Proof with auto.
+    intros ? ? c H; revert c.
+    induction 1.
+    - trivial.
+    - apply death_propagation...
+  Qed.
+
+
+  Lemma proper_death2 : 
+      forall {k1 k2}, context k1 k2 -> redex k2 -> ~ dead_ckind k1.
+
+  Proof with eauto.
+    intros k1 k2 c r H.
+    apply (proper_death k1)...
+  Qed.
+
+
+  Ltac inversion_ccons H :=
+
+      match type of H with ?ec1 =: ?c1  ~=  ?ec2 =: ?c2 => 
+
+      let H0 := fresh in 
+      assert (H0 : eq_dep _ _ _ (ec1=:c1) _ (ec2=:c2));
+
+      [ apply JMeq_eq_depT; eauto
+
+      | inversion H0; dep_subst; clear H0 ]
+
+      end.
+
+
+  Lemma plug_empty : forall t k, [.](k)[t] = t.
+  Proof.
+    intuition.
+  Qed.
+
+
+  Lemma compose_empty : forall {k1 k2} (c : context k1 k2), c = c ~+ [.].
+  Proof.
+    induction c.
+    - trivial.
+    - simpl; rewrite <- IHc; trivial.
+  Qed.
+
+
+  Lemma plug_compose  : 
+      forall {k1 k2 k3} (c0 : context k1 k2) (c1 : context k3 k1) t, 
+          (c0 ~+ c1)[t] = c1[c0[t]].
+  Proof.
+    induction c0; intros.
+    - auto.
+    - apply IHc0.
+  Qed.
+
+
+  Lemma context_cons_snoc : forall ec0 {k1 k2} (c0 : context k1 k2),
+                                exists ec1 c1, (ec0=:c0) = (c1~+ec1=:[.]).
+  Proof.
+    intros; revert ec0.
+    induction c0; intros.
+    - exists ec0; eexists [.]; trivial.
+    - destruct IHc0 with ec as (ec1, (c1, IH)).
+      exists ec1; eexists (ec0=:c1); rewrite IH; trivial.
+  Qed.
+
+
+End RED_LANG_Facts.
+
+
+
+
+Module RED_SEM_Facts (R : RED_LANG) (RS : RED_SEM R).
+
+  Module RF := RED_LANG_Facts R.
+  Import R.
+  Import RS.
+  Import RF.
+
+
+
+  Lemma dec_total : forall t k, ~ dead_ckind k -> 
+                        exists (d : decomp k), decempty t d.
+  Proof with eauto.
+    intros t k H.
+    destruct (decompose t k H) as [(v, H0) | (k', (r, (c, H0)))];
+        subst t.
+    - exists (d_val v). 
+      constructor.
+      apply dec_value_self...
+    - exists (d_red r c).
+      constructor.
+      apply dec_plug_rev.
+      + eapply (proper_death2 [.] r).
+      + rewrite <- compose_empty.
+        apply dec_redex_self.
+  Qed.
+
+End RED_SEM_Facts.
+
+
+
+(* Facts about a deterministic red. semantics.
+
+  Lemma unique_decomposition :
+
+      forall (t : term) k1, ~ dead_ckind k1 ->  
+
+         (exists v : value k1, t = v) \/
+
+         (exists k2 (r : redex k2) (c : context k1 k2), t = c[r] /\ 
+	      forall k2' (r' : redex k2') (c' : context k1 k2'), ~ dead_ckind k2' -> 
+                  t = c'[r'] -> k2' = k2 /\ r ~= r' /\ c ~= c').
+
+  Proof.
+    intros t k1 H.
+    destruct (dec_total t k1 H) as (d, H0); destruct H0.
+    destruct d.
+    - right.
+      exists k' r c.
+      split. apply (dec_correct H0).
+      intros k2' r' c' H1 H2.
+      assert (d_red r c = d_red r' c').
+      eapply dec_is_function. constructor.
+    apply H0.
+    subst.
+    apply dec_plug_rev. auto.
+    rewrite <- compose_empty.
+    apply dec_redex_self.
+    inversion H3; dep_subst.
+    auto.
+    - left. exists v. apply (dec_correct H0).
+  Qed. *)
+
