refocusing_machine_correct.v
@@ -1,0 +1,546 @@
+Require Import Util.
+Require Import Program.
+Require Import refocusing_semantics.
+Require Import refocusing_machine_sig.
+Require Import refocusing_machine.
+Require Import reduction_semantics_facts.
+Require Import refocusing_semantics_facts.
+
+
+
+Module PreAbstractMachine_Correct (R : RED_LANG) (RS : RED_REF_SEM R)
+                                  (PAM : PRE_ABSTRACT_MACHINE R RS). 
+
+  Import R.
+  Module RF := RED_LANG_Facts R.
+  Import RF.
+
+
+  Lemma dec_RS2PAM : forall {t k1 k2} {c : context k1 k2} {d}, 
+                         RS.dec t c d -> PAM.dec t c d.
+  Proof with eauto.
+    induction 1 using RS.dec_Ind with 
+    (P := fun t _ _ c d (_ : RS.dec t c d)    => PAM.dec t c d)
+    (P0:= fun _ v _ c d (_ : RS.decctx v c d) => PAM.decctx v c d);
+    solve 
+    [ econstructor; eauto
+    | eapply PAM.d_term; eauto
+    | eapply PAM.dc_term; eauto ].
+  Qed.
+
+
+  Lemma dec_PAM2RS : forall {t k1 k2} {c : context k1 k2} {d}, 
+                         PAM.dec t c d -> RS.dec t c d.
+  Proof with eauto.
+    induction 1 using PAM.dec_Ind with 
+    (P := fun t _ _ c d (_ : PAM.dec t c d)    => RS.dec t c d)
+    (P0:= fun _ v _ c d (_ : PAM.decctx v c d) => RS.decctx v c d);
+    solve
+    [ econstructor; eauto
+    | eapply RS.d_term; eauto
+    | eapply RS.dc_term; eauto ].
+  Qed.
+
+
+  Lemma dec_eqv: forall {t k1 k2} {c : context k1 k2} {d}, 
+                     RS.dec t c d <-> PAM.dec t c d.
+  Proof with auto using dec_RS2PAM, dec_PAM2RS.
+    intuition...
+  Qed.
+
+
+  Lemma iter_RS2PAM : forall {k} {d : decomp k} {v}, 
+                          RS.RS.iter d v -> PAM.iter d v.
+  Proof with eauto.
+    induction 1.
+    - constructor...
+    - econstructor...
+      dependent destruction H0.
+      apply dec_RS2PAM.
+      apply RS.RS.dec_plug in H0.
+      + erewrite (compose_empty _)...
+      + eapply (proper_death2 [.])...
+  Qed.
+
+
+  Lemma iter_PAM2RS : forall {k} {d : decomp k} {v}, 
+                          PAM.iter d v -> RS.RS.iter d v.
+  Proof with eauto.
+    induction 1.
+    - constructor.
+    - econstructor...
+      constructor.
+      apply RS.RS.dec_plug_rev.
+      + eapply (proper_death2 [.])...
+      + rewrite <- compose_empty...
+        apply dec_PAM2RS...
+  Qed.
+
+
+  Lemma iter_eqv : forall {k} {d : decomp k} {v}, 
+                       RS.RS.iter d v <-> PAM.iter d v.
+
+  Proof with auto using iter_RS2PAM, iter_PAM2RS.
+    intuition...
+  Qed.
+
+
+  Lemma eval_RS2PAM : forall {t v}, RS.RS.eval t v -> PAM.eval t v.
+  Proof with eauto.
+    intros t v H.
+    dependent destruction H; econstructor.
+    - dependent destruction H.
+      apply dec_RS2PAM...
+    - apply iter_RS2PAM...
+  Qed.
+
+
+  Lemma eval_PAM2RS : forall {t v}, PAM.eval t v -> RS.RS.eval t v.
+  Proof with eauto.
+    intros t v H.
+    dependent destruction H; econstructor.
+    - constructor.
+      eapply dec_PAM2RS...
+    - apply iter_PAM2RS...
+  Qed.
+
+
+  Theorem eval_OK : forall {t v} , RS.RS.eval t v <-> PAM.eval t v.
+
+  Proof with auto using eval_PAM2RS, eval_RS2PAM.
+    intuition...
+  Qed.
+
+End PreAbstractMachine_Correct.
+
+
+
+
+Module StagedAbstractMachine_Correct (R : RED_LANG) (RS : RED_REF_SEM R)
+                                     (SAM : STAGED_ABSTRACT_MACHINE R RS).
+
+  Module RF   := RED_LANG_Facts R.
+  Module RSF  := RED_SEM_Facts R RS.RS.
+  Module RSD  := RedRefSemDet R RS.
+  Module PAM := PreAbstractMachine R RS.
+  Module PAMC := PreAbstractMachine_Correct R RS PAM.
+  Import R.
+  Import RF.
+  Import RSF.
+
+
+
+  Lemma dec_PAM2SAM : forall {t k1 k2} {c : context k1 k2} {d v},
+                          PAM.dec t c d -> SAM.iter d v -> SAM.dec t c v.
+  Proof with eauto.
+    induction 1 using PAM.dec_Ind with
+    (P  := fun t _ _ c d (_ : PAM.dec t c d)    => 
+               forall v,  SAM.iter d v  -> SAM.dec t c v)
+    (P0 := fun _ v _ c d (_ : PAM.decctx v c d) => 
+               forall v', SAM.iter d v' -> SAM.decctx v c v');
+    intros; simpl; solve 
+    [ econstructor; eauto
+    | eapply SAM.d_v; eauto
+    | eapply SAM.d_many; eauto 
+    | eapply SAM.dc_val; eauto
+    | eapply SAM.dc_term; eauto ].
+  Qed.
+
+
+  Lemma dec_SAM2PAM : forall {t k1 k2} {c : context k1 k2} {d v},
+                          SAM.dec t c v -> PAM.dec t c d -> PAM.iter d v.
+
+  Proof with eauto using proper_death2, (proper_death2 [.]).
+    intros t k1 k2 c d v H; revert d.
+
+    induction H using SAM.dec_Ind with
+    (P  := fun t _ _ c v  (_ : SAM.dec t c v)     => 
+               forall d, PAM.dec t c d -> PAM.iter d v)
+    (P0 := fun _ v _ c v' (_ : SAM.decctx v c v') => 
+               forall d, PAM.decctx v c d -> PAM.iter d v')
+    (P1 := fun _ d v      (_ : SAM.iter d v)      => 
+               PAM.iter d v);
+
+        try (intros d0 G; 
+             dependent destruction G; 
+             try match goal with H : _ =: _ ~= _ =: _ |- _ => inversion_ccons H end);
+
+    try solve 
+    [ constructor
+
+    | eauto
+
+    | match goal       with H0 : ?x = ?d0,  H1 : ?x = ?d1 |- _ => 
+      match type of d0 with SAM.DEC.interm_dec _ => 
+          rewrite H0 in H1; inversion H1; subst; eauto 
+      end end ].
+
+    (* the last case *)
+    - destruct (dec_total c[t] k1) as (d, H0)...
+      assert (PAM.dec t c d).
+      {
+          rewrite <- PAMC.dec_eqv.
+          dependent destruction H0.
+          apply RS.RS.dec_plug in H0...
+          rewrite <- compose_empty in H0.
+          assumption.
+      }
+      econstructor...
+  Qed.
+
+
+  Lemma iter_PAM2SAM : forall {k} {d : decomp k} {v}, PAM.iter d v -> SAM.iter d v.
+
+  Proof with eauto using dec_PAM2SAM.
+    induction 1; [ constructor 1 | econstructor 2 ]...
+  Qed.
+
+
+  Lemma eval_PAM2SAM : forall {t} {v : value init_ckind}, PAM.eval t v -> SAM.eval t v.
+
+  Proof with eauto using iter_PAM2SAM, dec_PAM2SAM.
+    intros t v H; dependent destruction H; constructor...
+  Qed.
+
+
+  Lemma eval_SAM2PAM : forall {t v}, SAM.eval t v -> PAM.eval t v.
+
+  Proof with eauto using (proper_death2 [.]), PAMC.dec_eqv.
+    intros t v H.
+    dependent destruction H.
+    destruct (dec_total t init_ckind) as (d, H0).
+    - dependent destruction H...
+      + inversion H0; dep_subst...
+      + intro G; rewrite SAM.DEC.dec_term_from_dead in H...
+    - dependent destruction H0. econstructor...
+      + eapply PAMC.dec_eqv...
+      + eapply dec_SAM2PAM...
+        apply PAMC.dec_eqv...
+  Qed.
+
+
+  Theorem eval_OK : forall {t v}, RS.RS.eval t v <-> SAM.eval t v.
+
+  Proof with auto using PAMC.eval_OK, eval_SAM2PAM, eval_PAM2SAM.
+    etransitivity...
+    intuition...
+  Qed.
+
+End StagedAbstractMachine_Correct.
+
+
+
+
+Module EvalApplyMachine_Correct (R : RED_LANG) (RS : RED_REF_SEM R)
+                                (EAM : EVAL_APPLY_MACHINE R RS).
+
+  Module SAM  := StagedAbstractMachine R RS.
+  Module SAMC := StagedAbstractMachine_Correct R RS SAM.
+  Import R.
+  Import RS.
+  Export DEC.
+
+
+
+  Local Hint Constructors EAM.dec EAM.decctx EAM.eval.
+
+  Lemma dec_SAM2EAM : forall {t k1 k2} {c : context k1 k2} {v}, 
+                          SAM.dec t c v -> EAM.dec t c v.
+  Proof.
+    intros t k1 k2 c v.
+
+    induction 1 using SAM.dec_Ind with
+    (P := fun t _ _ c v  (_ : SAM.dec t c v)     => EAM.dec t c v)
+    (P0:= fun _ v _ c v' (_ : SAM.decctx v c v') => EAM.decctx v c v')
+    (P1:= fun k d v      (_ : SAM.iter d v)      => 
+              match d with
+              | d_val v'    => ~ dead_ckind k -> EAM.decctx v [.] v'
+              | d_red _ r c => forall t, contract r = Some t -> EAM.dec t c v
+              end);
+        intros;
+
+    match goal with 
+
+    | _ => solve [eauto]
+
+    | H : SAM.iter _ _ |- _ => 
+          inversion H; dep_subst; 
+          solve [eauto] 
+
+    | H0 : contract ?r = ?t0 , H1 : contract ?r = ?t1 |- _ =>
+          rewrite H0 in H1; 
+          inversion H1; subst; 
+          solve [eauto]
+    end.
+  Qed.
+
+
+  Local Hint Constructors SAM.dec SAM.decctx SAM.iter SAM.eval.
+
+  Lemma dec_EAM2SAM : forall {t k1 k2} {c : context k1 k2} {v}, 
+                          EAM.dec t c v -> SAM.dec t c v.
+  Proof with eauto.
+    induction 1 using EAM.dec_Ind with
+    (P := fun t _ _ c v  (_ : EAM.dec t c v)     => SAM.dec t c v)
+    (P0:= fun _ v _ c v' (_ : EAM.decctx v c v') => SAM.decctx v c v')
+    ...
+  Qed.
+
+
+  Lemma eval_SAM_EAM : forall {t v}, SAM.eval t v <-> EAM.eval t v.
+
+  Proof.
+    split; 
+
+    solve
+    [ intro H;
+      dependent destruction H; 
+      eauto using dec_SAM2EAM, dec_EAM2SAM ].
+  Qed.
+
+
+  Theorem eval_OK : forall {t v}, RS.RS.eval t v <-> EAM.eval t v.
+  Proof with eauto using SAMC.eval_OK, eval_SAM_EAM.
+    etransitivity...
+  Qed.
+
+End EvalApplyMachine_Correct.
+
+
+
+
+Module ProperEAMachine_Correct (R : RED_LANG) (RS : RED_REF_SEM R) 
+                               (PEAM : PROPER_EA_MACHINE R RS).
+
+  Module EAM  := EvalApplyMachine R RS.
+  Module EAMC := EvalApplyMachine_Correct R RS EAM.
+  Import R.
+  Import RS.DEC.
+  Import PEAM.
+
+
+  Local Hint Constructors PEAM.trans PEAM.trans_close.
+
+  Lemma dec_EAM2PEAM : forall {t k1 k2} (c : context k1 k2) {v}, 
+                           EAM.dec t c v -> c_eval t c →+ c_apply [.] v.
+  Proof with eauto.
+    induction 1 using EAM.dec_Ind with
+    (P := fun t _ _ c v  (_ : EAM.dec t c v)     => 
+              c_eval t c  →+ c_apply [.] v)
+    (P0:= fun k2 v k1 c v' (_ : EAM.decctx v c v') => 
+              c_apply c v →+ c_apply [.] v' \/ k1 = k2 /\ [.](k1) ~= c /\ v ~=v');
+
+    intuition; dep_subst...
+  Qed.
+
+
+  Lemma eval_EAM2PEAM : forall {t v}, 
+                            EAM.eval t v -> PEAM.eval t v.
+  Proof with eauto using dec_EAM2PEAM.
+    intros t v H.
+    dependent destruction H; constructor...
+  Qed.
+
+
+  Local Hint Constructors EAM.dec EAM.decctx.
+
+  Lemma trans_PEAM2EAM : forall {t k1 k2} {c : context k1 k2} {v}, 
+                             c_eval t c →+ c_apply [.] v -> EAM.dec t c v.
+  Proof with eautof.
+    intros t k1 k2 c v; revert t k2 c.
+
+    cut (forall co, co →+ c_apply [.] v -> 
+         match co with 
+         | c_eval t k1' _ c   => k1 = k1' -> forall v', v ~= v' -> EAM.dec t c v'
+         | c_apply k1' _ c v0 => k1 = k1' -> forall v', v ~= v' -> EAM.decctx v0 c v'
+         end).
+    {
+        intros H t k2 c H0; apply (H _ H0)...
+    }
+
+    intros co H.
+
+    dependent induction H;
+        match goal with H : transition _ _ |- _ => 
+              dependent_destruction2 H end;
+        match goal with 
+        | H : dec_term _ ?k = _ |- _=> 
+              assert (~ dead_ckind k);
+              [ intro; rewrite dec_term_from_dead in H; solve[eauto] 
+              | ]
+        | H : dec_context _ ?k _ = _ |- _=> 
+              assert (~ dead_ckind k);
+              [ intro; rewrite dec_context_from_dead in H; 
+                solve [eauto using death_propagation] 
+              | ]
+        end;
+
+    intros; dep_subst...
+  Qed.
+
+  
+  Lemma eval_PEAM2EAM : forall {t v}, PEAM.eval t v -> EAM.eval t v.
+
+  Proof with eauto using trans_PEAM2EAM.
+    intros.
+    dependent destruction H; constructor...
+  Qed.
+
+
+  Theorem eval_OK : forall {t v}, RS.RS.eval t v <-> PEAM.eval t v.
+  Proof with auto using EAMC.eval_OK, eval_PEAM2EAM, eval_EAM2PEAM.
+    etransitivity...
+    intuition...
+  Qed.
+
+End ProperEAMachine_Correct.
+
+
+
+
+Module PushEnterMachine_Correct (R : RED_LANG) (PERS : PE_REF_SEM R) 
+                                (PEM : PUSH_ENTER_MACHINE R PERS).
+
+  Module RS   := PERS.RefSem.
+  Module EAM  := EvalApplyMachine R PERS.RefSem.
+  Module EAMC := EvalApplyMachine_Correct R PERS.RefSem EAM.
+  Import R.
+  Import PEM.DEC.
+
+
+
+  Local Hint Constructors PEM.dec EAM.dec EAM.decctx.
+
+  Lemma dec_EAM2PEM : forall {t k1 k2} {c : context k1 k2} {v}, 
+                          EAM.dec t c v -> PEM.dec t c v.
+  Proof with eauto.
+    induction 1 using EAM.dec_Ind with
+    (P := fun t _ _ c v  (_ : EAM.dec t c v) => PEM.dec t c v)
+    (P0:= fun _ v _ c v0 (_ : EAM.decctx v c v0) =>
+      match c in context _ k2' return value k2' -> Prop with
+      | [.] => fun v => PEM.dec v [.] v0
+      | ccons ec _ c => fun v => forall d, dec_context ec _ v = d ->
+        match d with
+        | PEM.DEC.in_red r => forall t, contract r = Some t -> PEM.dec t c v0
+        | in_term t ec0 => PEM.dec t (ec0=:c) v0
+        | in_val v => False
+        | in_dead => False
+        end
+      end v); intros...
+
+    - dependent destruction d; subst...
+      + eapply PEM.dec_red...
+        eapply (IHdec (in_red _))...
+      + contradict (PERS.dec_context_not_val _ _ _ H).
+      + eapply PEM.dec_v_t...
+        eapply (IHdec (in_term _ _))...
+
+    - constructor; apply PERS.dec_term_value...
+
+    - rewrite e in H0;  inversion H0; subst.
+      intros.
+      rewrite e0 in H0; inversion H0; subst...
+
+    - contradict (PERS.dec_context_not_val _ _ _ e).
+
+    - rewrite e in H0; subst...
+  Qed.
+
+
+  Lemma dec_PEM2EAM : forall {t k1 k2} {c : context k1 k2} {v}, 
+                          PEM.dec t c v -> EAM.dec t c v.
+  Proof with eauto.
+    induction 1...
+    - assert (~ dead_ckind k).
+      {
+          intro; rewrite dec_term_from_dead in *; autof.
+      }
+      eauto.
+  Qed.
+
+
+
+  Lemma eval_EAM2PEM : forall {t v}, EAM.eval t v -> PEM.eval t v.
+
+  Proof with eauto using dec_EAM2PEM.
+    intros t v H.
+    dependent destruction H; constructor...
+  Qed.
+
+
+  Lemma eval_PEM2EAM : forall {t v}, PEM.eval t v -> EAM.eval t v.
+
+  Proof with eauto using dec_PEM2EAM.
+    intros t v H.
+    dependent destruction H; constructor...
+  Qed.
+
+
+  Theorem eval_OK : forall {t v}, RS.RS.eval t v <-> PEM.eval t v.
+  Proof with eauto using EAMC.eval_OK, eval_PEM2EAM, eval_EAM2PEM.
+    etransitivity...
+    intuition...
+  Qed.
+
+End PushEnterMachine_Correct.
+
+
+
+
+Module ProperPEMachine_Correct (R : RED_LANG) (PRS : PE_REF_SEM R) 
+                               (PPEM : PROPER_PE_MACHINE R PRS).
+
+  Module RS   := PRS.RefSem.
+  Module PEM  := PushEnterMachine R PRS.
+  Module PEMC := PushEnterMachine_Correct R PRS PEM.
+  Import R.
+  Import RS.DEC.
+  Import PPEM.
+
+
+
+  Local Hint Constructors PPEM.trans PPEM.trans_close PEM.dec.
+
+  Lemma dec_PEM2PPEM : forall {t} {k1 k2} {c : context k1 k2} {v}, 
+                           PEM.dec t c v -> c_eval t c →+ c_fin v.
+  Proof with eauto.
+    induction 1...
+  Qed.
+
+
+  Lemma eval_PEM2PPEM : forall {t v}, PEM.eval t v -> PPEM.eval t v.
+
+  Proof with eauto using dec_PEM2PPEM.
+    intros t v H.
+    dependent destruction H; constructor...
+  Qed.
+
+
+  Lemma trans_PPEM2PEM : forall {t k1 k2} {c : context k1 k2} {v}, 
+                             c_eval t c →+ c_fin v -> PEM.dec t c v.
+  Proof with eauto.
+    intros t k1 k2 c v H.
+    dependent induction H;
+        match goal with H : transition _ _ |- _ => 
+            dependent_destruction2 H end;
+    solve 
+    [ eauto 
+    | inversion H0 as [? ? H | ? ? ? H ]; inversion H ].
+  Qed.
+
+
+  Lemma eval_PPEM2PEM : forall {t v}, PPEM.eval t v -> PEM.eval t v.
+
+  Proof with eauto using trans_PPEM2PEM.
+    intros t v H.
+    destruct H; constructor...
+  Qed.
+
+
+  Theorem eval_OK : forall {t v}, RS.RS.eval t v <-> PPEM.eval t v.
+  Proof with eauto using PEMC.eval_OK, eval_PEM2PPEM, eval_PPEM2PEM.
+    etransitivity...
+    intuition...
+  Qed.
+
+End ProperPEMachine_Correct.
