refocusing_semantics.v
@@ -1,10 +1,12 @@
 Require Export reduction_semantics.
+Require Export refocusing_step.
 
 
+(* Refocusing semantics *)
 
 Module Type RED_REF_SEM (R : RED_LANG).
 
-  Declare Module DEC : DEC_STEP R.
+  Declare Module DEC : REF_STEP R.
   Import R.
   Export DEC.
 
@@ -59,146 +61,8 @@ End RED_REF_SEM.
 
 
 
-Require Import Util.
-Require Import Program.
-Require Import reduction_lang_facts.
 
-
-Module Red_Sem_Proper (R : RED_LANG) (RS : RED_REF_SEM R) : RED_SEM_PROPER R RS.RS.
-
-  Import R.
-  Module RLF := RED_LANG_Facts R.
-  Import RLF.
-  Import RS.
-  Export DEC.
-
-
-  Lemma dec_is_function : forall {t k} {d d0 : decomp k}, 
-                              decempty t d -> decempty t d0 -> d = d0.
-  Proof.
-    intros t k d1 d2 DE1 DE2.
-    dependent destruction DE1; dependent destruction DE2.
-
-    induction H using dec_Ind with 
-    (P  := fun t _ _ c d _ => forall d0, dec t c d0    -> d = d0)
-    (P0 := fun _ v _ c d _ => forall d0, decctx v c d0 -> d = d0);
-
-    intros;
-
-    (* automated cases *)
-    match goal with
-
-    | [ RD : (dec ?t ?c ?d), DT1 : (dec_term ?t ?k = _) |- _ ] => 
-             inversion RD; dep_subst; 
-             match goal with DT2 : (dec_term ?t ?k = _) |- _ => 
-                 rewrite DT2 in DT1; inversion DT1 end
-
-    | [ RC : (decctx ?v (?ec=:?c) ?d), DC1 : (dec_context ?ec ?k ?v = _) |- _ ] => 
-             dependent_destruction2 RC; inversion_ccons x2; dep_subst;
-             match goal with DC2 : (dec_context ?ec' ?k' ?v' = _) |- _ => 
-                 rewrite DC2 in DC1; inversion DC1 end
-
-    | [ RC : (decctx ?v [.] ?d) |- _] => 
-             dependent_destruction2 RC
-
-    end;
-
-    subst; eauto.
-  Qed.
-  Hint Resolve dec_is_function : prop.
-
-
-  Lemma iter_is_function : forall {k} {d : decomp k} {v v0}, 
-                               iter d v -> iter d v0 -> v = v0.
-  Proof with eauto with prop.
-    induction 1; intros.
-    - dependent destruction H...
-    - dependent destruction H2; subst. 
-      rewrite H2 in H; inversion H; subst.
-      apply IHiter.
-      cutrewrite (d = d0)...
-  Qed.
-  Hint Resolve iter_is_function : prop.
-
-
-  Lemma eval_is_function : forall {t} {v v0 : value init_ckind}, 
-                               eval t v -> eval t v0 -> v = v0.
-  Proof with eauto with prop.
-    intros.
-    dependent destruction H.
-    dependent destruction H1.
-    cutrewrite (d = d0) in H0...
-  Qed.
-
-
-  Lemma dec_correct : forall {t k1 k2} {c : context k1 k2} {d}, 
-                          dec t c d -> decomp_to_term d = c[t].
-  Proof.
-    induction 1 using dec_Ind with
-    (P := fun t _ _ c d (H : dec t c d)     => decomp_to_term d = c[t])
-    (P0:= fun _ v _ c d (H:RS.decctx v c d) => decomp_to_term d = c[v]);
-    simpl; auto;
-
-    first
-    [ assert (G := dec_term_correct t k2);       rewrite e in G
-    | assert (G := dec_context_correct ec k2 v); rewrite e in G ]; 
-    
-    simpl in *; 
-    try rewrite IHdec;
-    congruence.
-  Qed.
-
-
-  Lemma dec_total : forall t k, ~ dead_ckind k -> exists (d : decomp k), decempty t d.
-  Proof with auto.
-    intros t k H.
-    destruct (decompose t k H) as [(v, ?) | (?, (r, (c, ?)))]; 
-    intros; subst.
-    - exists (d_val v); constructor.
-      rewrite dec_val_self.
-      constructor...
-    - exists (d_red r c); constructor.
-      apply dec_plug_rev.
-        { apply (proper_death2 _ _ [.] r). }
-      rewrite <- compose_empty.
-      apply dec_redex_self.
-  Qed.
-
-
-  Lemma unique_decomposition :
-
-      forall (t : term) k1, ~ dead_ckind k1 ->
-          (exists v : value k1, t = v) \/ 
-          (exists k2 (r : redex k2) (c : context k1 k2),  t = c[r] /\ 
-	      forall k2' (r0 : redex k2') (c0 : context k1 k2'), 
-                  t = c0[r0] -> k2' = k2 /\ r ~= r0 /\ c ~= c0).
-
-  Proof with eauto.
-    intros.
-    destruct (decompose t k1 H) as [(v, H0) | (k', (r, (c, H0)))].
-    - left; exists v...
-    - right; exists k' r; exists c; split.
-      + congruence.
-      + intros.
-        assert (H2 : decempty t (d_red r c) /\ decempty t (d_red r0 c0)).
-        {
-            split;
-            constructor; 
-            [ rewrite H0 | rewrite H1 ]; 
-            apply dec_plug_rev;
-            solve
-            [ apply (proper_death2 _ _ [.]); auto
-            | rewrite <- compose_empty; apply dec_redex_self ]. 
-        }
-        destruct H2.
-        assert (H4 := dec_is_function H2 H3); dependent destruction H4.
-        intuition.
-  Qed.
-
-End Red_Sem_Proper.
-
-
-
+(* Push-enter refocusing semantics *)
 
 Module Type PE_REF_SEM (R : RED_LANG).
 
@@ -207,7 +71,8 @@ Module Type PE_REF_SEM (R : RED_LANG).
   Export RefSem.
 
   Axiom dec_context_not_val : 
-      forall ec {k} v (v0 : value k), dec_context ec k v <> in_val v0.
+      forall ec {k} v1 (v0 : value (k+>ec)), dec_context ec k v0 <> in_val v1.
+
   Axiom dec_term_value : 
       forall {k} (v : value k), dec_term v k = in_val v.
 
